

The Inverse of a Partitioned Matrix

Zongwu Cai, Department of Economics, University of Kansas

February 27, 2024

Consider a pair A, B of $n \times n$ matrices, partitioned as

$$A = \begin{pmatrix} A_{11} & A_{12} \\ A_{21} & A_{22} \end{pmatrix} \quad \text{and} \quad B = \begin{pmatrix} B_{11} & B_{12} \\ B_{21} & B_{22} \end{pmatrix},$$

where A_{11} and B_{11} are $k \times k$ matrices. Suppose that A is nonsingular and $B = A^{-1}$. In this note it will be shown how to derive the B_{ij} 's in terms of the A_{ij} 's, given that

$$\det(A_{11}) \neq 0 \quad \text{and} \quad \det(A_{22}) \neq 0. \quad (1)$$

If $B = A^{-1}$, then,

$$\begin{aligned} AB &= \begin{pmatrix} A_{11} & A_{12} \\ A_{21} & A_{22} \end{pmatrix} \begin{pmatrix} B_{11} & B_{12} \\ B_{21} & B_{22} \end{pmatrix} \\ &= \begin{pmatrix} A_{11}B_{11} + A_{12}B_{21} & A_{11}B_{12} + A_{12}B_{22} \\ A_{21}B_{11} + A_{22}B_{21} & A_{21}B_{12} + A_{22}B_{22} \end{pmatrix} \\ &= \begin{pmatrix} I_k & O_{k,n-k} \\ O_{n-k,k} & I_{n-k} \end{pmatrix}, \end{aligned} \quad (2)$$

where as usual I denotes the unit matrix and O a zero matrix, with sizes indicated by the subscripts involved. To solve (2), we need to solve four matrix equations:

$$A_{11}B_{11} + A_{12}B_{21} = I_k, \quad (3)$$

$$A_{11}B_{12} + A_{12}B_{22} = O_{k,n-k}, \quad (4)$$

$$A_{21}B_{11} + A_{22}B_{21} = O_{n-k,k} \quad (5)$$

$$A_{21}B_{12} + A_{22}B_{22} = I_{n-k} \quad (6)$$

It follows from (4) and (5) that

$$B_{12} = -A_{11}^{-1}A_{12}B_{22}, \quad (7)$$

$$B_{21} = -A_{22}^{-1}A_{21}B_{11}, \quad (8)$$

so that (3) and (6) become

$$\begin{aligned} (A_{11} - A_{12}A_{22}^{-1}A_{21})B_{11} &= I_k, \\ (A_{22} - A_{21}A_{11}^{-1}A_{12})B_{22} &= I_{n-k}. \end{aligned}$$

Hence,

$$\begin{aligned} B_{11} &= (A_{11} - A_{12}A_{22}^{-1}A_{21})^{-1} \\ B_{22} &= (A_{22} - A_{21}A_{11}^{-1}A_{12})^{-1}. \end{aligned}$$

Substituting these solutions in (7) and (8) it follows that

$$\begin{aligned} B_{12} &= -A_{11}^{-1}A_{12} (A_{22} - A_{21}A_{11}^{-1}A_{12})^{-1} \\ B_{21} &= -A_{22}^{-1}A_{21} (A_{11} - A_{12}A_{22}^{-1}A_{21})^{-1}. \end{aligned}$$

Thus,

$$A^{-1} = \begin{pmatrix} (A_{11} - A_{12}A_{22}^{-1}A_{21})^{-1} & -A_{11}^{-1}A_{12} (A_{22} - A_{21}A_{11}^{-1}A_{12})^{-1} \\ -A_{22}^{-1}A_{21} (A_{11} - A_{12}A_{22}^{-1}A_{21})^{-1} & (A_{22} - A_{21}A_{11}^{-1}A_{12})^{-1} \end{pmatrix}.$$

Moreover, since $AA^{-1} = I_n$ implies $A^{-1}A = I_n$, we also have

$$A^{-1} = \begin{pmatrix} (A_{11} - A_{12}A_{22}^{-1}A_{21})^{-1} & -(A_{11} - A_{12}A_{22}^{-1}A_{21})^{-1}A_{12}A_{22}^{-1} \\ -(A_{22} - A_{21}A_{11}^{-1}A_{12})^{-1}A_{21}A_{11}^{-1} & (A_{22} - A_{21}A_{11}^{-1}A_{12})^{-1} \end{pmatrix}.$$